Revision of the narrative in Dimensions and Quantities

src/SI/ISQ_Quantities.thy
@@ -4,16 +4,27 @@ theory ISQ_Quantities
   imports ISQ_Dimensions
 begin
 
-section \<open> The Semantic SI-Unit-Type and its Operations \<close>
+section \<open> Quantity Semantic Domain \<close>
+
+text \<open> Here, we give a semantic domain for particular values of physical quantities. A quantity 
+  is usually expressed as a number and a measurement unit, and the goal is to support this. First,
+  though, we give a more general semantic domain where a quantity has a magnitude and a dimension. \<close>
 
 record 'a Quantity =
-  mag  :: 'a        \<comment> \<open> Magnitude of the unit \<close>
-  dim  :: Dimension \<comment> \<open> Dimension of the unit \<close>
+  mag  :: 'a        \<comment> \<open> Magnitude of the quantity. \<close>
+  dim  :: Dimension \<comment> \<open> Dimension of the quantity -- denote the kind of quantity. \<close>
+
+text \<open> The quantity type is parametric as we permit the magnitude to be represented using any kind 
+  of numeric type, such as \<^typ>\<open>int\<close>, \<^typ>\<open>rat\<close>, or \<^typ>\<open>real\<close>, though we usually minimally expect
+  a field. \<close>
 
 lemma Quantity_eq_intro:
   assumes "mag x = mag y" "dim x = dim y" "more x = more y"
   shows "x = y"
   by (simp add: assms)
+
+text \<open> We can define several arithmetic operators on quantities. Multiplication takes multiplies
+  both the magnitudes and the dimensions. \<close>
 
 instantiation Quantity_ext :: (times, times) times
 begin
@@ -25,6 +36,9 @@ end
 lemma mag_times  [simp]: "mag (x \<cdot> y) = mag x \<cdot> mag y" by (simp add: times_Quantity_ext_def)
 lemma dim_times  [simp]: "dim (x \<cdot> y) = dim x \<cdot> dim y" by (simp add: times_Quantity_ext_def)
 lemma more_times [simp]: "more (x \<cdot> y) = more x \<cdot> more y" by (simp add: times_Quantity_ext_def)
+
+text \<open> The zero and one quantities are both dimensionless quantities with magnitude of \<^term>\<open>0\<close> and
+  \<^term>\<open>1\<close>, respectively. \<close>
 
 instantiation Quantity_ext :: (zero, zero) zero
 begin
@@ -45,6 +59,9 @@ end
 lemma mag_one  [simp]: "mag 1 = 1" by (simp add: one_Quantity_ext_def)
 lemma dim_one  [simp]: "dim 1 = 1" by (simp add: one_Quantity_ext_def)
 lemma more_one [simp]: "more 1 = 1" by (simp add: one_Quantity_ext_def)
+
+text \<open> Quantity inversion inverts both the magnitude and the dimension. Similarly, division of
+  one quantity by another, divides both the magnitudes and the dimensions. \<close>
 
 instantiation Quantity_ext :: (inverse, inverse) inverse
 begin
@@ -73,12 +90,16 @@ lemma dim_divide [simp]: "dim (x / y) = dim x / dim y"
 lemma more_divide [simp]: "more (x / y) = more x / more y" 
   by (simp add: divide_Quantity_ext_def)
 
+text \<open> As for dimensions, quantities form a commutative monoid and an abelian group. \<close>
+
 instance Quantity_ext :: (comm_monoid_mult, comm_monoid_mult) comm_monoid_mult
   by (intro_classes, simp_all add: one_Quantity_ext_def 
                                    times_Quantity_ext_def mult.assoc, simp add: mult.commute)
 
 instance Quantity_ext :: (ab_group_mult, ab_group_mult) ab_group_mult
   by (intro_classes, rule Quantity_eq_intro, simp_all)
+
+text \<open> We can also define a partial order on quantities. \<close>
 
 instantiation Quantity_ext :: (ord, ord) ord
 begin
@@ -94,39 +115,68 @@ end
 instance Quantity_ext :: (order, order) order
   by (intro_classes, auto simp add: less_Quantity_ext_def less_eq_Quantity_ext_def)
 
-section \<open> The Abstract SI-\<^theory_text>\<open>Quantity\<close>-Type and its Operations \<close>
+text \<open> We can define plus and minus as well, but these are partial operators as they are defined
+  only when the quantities have the same dimension. \<close>
 
-text\<open>We 'lift' SI type expressions to SI unit type expressions as follows:\<close>
+instantiation Quantity_ext :: (plus, plus) plus
+begin
+  definition [si_def]:
+    "dim x = dim y \<Longrightarrow> 
+     plus_Quantity_ext x y = \<lparr> mag = mag x + mag y, dim = dim x, \<dots> = more x + more y \<rparr>"
+instance ..
+end
 
-typedef (overloaded) ('n, 'u::dim_type) QuantT ("_[_]" [999,0] 999) 
-                     = "{x :: 'n Quantity. dim x = QD('u)}"
-  morphisms fromQ toQ by (rule_tac x="\<lparr> mag = undefined, dim = QD('u) \<rparr>" in exI, simp)
+instantiation Quantity_ext :: (uminus, uminus) uminus
+begin
+  definition [si_def]:
+    "uminus_Quantity_ext x = \<lparr> mag = - mag x , dim = dim x, \<dots> = - more x \<rparr>"
+instance ..
+end
+
+instantiation Quantity_ext :: (minus, minus) minus
+begin
+  definition [si_def]:
+    "dim x = dim y \<Longrightarrow> 
+      minus_Quantity_ext x y = \<lparr> mag = mag x - mag y, dim = dim x, \<dots> = more x - more y \<rparr>"
+instance ..
+end
+
+section \<open> Dimension Typed Quantities \<close>
+
+text \<open> We can now define the type of quantities with parametrised dimension types. \<close>
+
+typedef (overloaded) ('n, 'd::dim_type) QuantT ("_[_]" [999,0] 999) 
+                     = "{x :: 'n Quantity. dim x = QD('d)}"
+  morphisms fromQ toQ by (rule_tac x="\<lparr> mag = undefined, dim = QD('d) \<rparr>" in exI, simp)
 
 setup_lifting type_definition_QuantT
 
-text \<open> Coerce values when their dimensions are equivalent \<close>
+text \<open> A dimension typed quantity is parameterised by two types: \<^typ>\<open>'a\<close>, the numeric type for the
+  magntitude, and \<^typ>\<open>'d\<close> for the dimension expression, which is an element of \<^class>\<open>dim_type\<close>. 
+  The type \<^typ>\<open>('n, 'd) QuantT\<close> is to \<^typ>\<open>'n Quantity\<close> as dimension types are to \<^typ>\<open>Dimension\<close>. 
+  Specifically, an element of \<^typ>\<open>('n', 'd) QuantT\<close> is a quantity whose dimension is \<^typ>\<open>'d\<close>. \<close>
 
-definition coerceQuantT :: "'u\<^sub>2 itself \<Rightarrow> 'a['u\<^sub>1::dim_type] \<Rightarrow> 'a['u\<^sub>2::dim_type]" where
-"QD('u\<^sub>1) = QD('u\<^sub>2) \<Longrightarrow> coerceQuantT t x = (toQ (fromQ x))"
+text \<open> Since quantities can have dimension type expressions that are distinct, but denote the same
+  dimension, it is necessary to define the following function for coercion between two dimension
+  expressions. This requires that the underlying dimensions are the same. \<close>
 
-subsection\<open>Predicates on Abstract SI-\<^theory_text>\<open>Unit\<close>-types\<close>
+definition coerceQuantT :: "'d\<^sub>2 itself \<Rightarrow> 'a['d\<^sub>1::dim_type] \<Rightarrow> 'a['d\<^sub>2::dim_type]" where
+"QD('d\<^sub>1) = QD('d\<^sub>2) \<Longrightarrow> coerceQuantT t x = (toQ (fromQ x))"
+
+subsection \<open> Predicates on Typed Quantities \<close>
 
 text \<open> Two SI Unit types are orderable if their magnitude type is of class @{class "order"},
        and have the same dimensions (not necessarily dimension types).\<close>
 
-lift_definition qless_eq :: 
-                "'n::order['a::dim_type] \<Rightarrow> 'n['b::dim_type] \<Rightarrow> bool" (infix "\<lesssim>\<^sub>Q" 50) is "(\<le>)" .
-
+lift_definition qless_eq :: "'n::order['a::dim_type] \<Rightarrow> 'n['b::dim_type] \<Rightarrow> bool" (infix "\<lesssim>\<^sub>Q" 50) 
+  is "(\<le>)" .
 
 text\<open> Two SI Unit types are equivalent if they have the same dimensions
       (not necessarily dimension types). This equivalence the a vital point 
       of the overall construction of SI Units. \<close>
 
-lift_definition qequiv ::
-                "'n['a::dim_type] \<Rightarrow> 'n['b::dim_type] \<Rightarrow> bool" (infix "\<cong>\<^sub>Q" 50) is  "(=)" .
-
-subsection\<open>The Equivalence on Abstract SI-\<^theory_text>\<open>Unit\<close>-Types\<close>
-text\<open>The latter predicate gives us an equivalence, but, unfortunately, not a congruence.\<close>
+lift_definition qequiv :: "'n['a::dim_type] \<Rightarrow> 'n['b::dim_type] \<Rightarrow> bool" (infix "\<cong>\<^sub>Q" 50) 
+  is "(=)" .
 
 lemma qequiv_refl [simp]: "a \<cong>\<^sub>Q a"
   by (simp add: qequiv_def)
@@ -138,49 +188,49 @@ lemma qequiv_trans: "\<lbrakk> a \<cong>\<^sub>Q b; b \<cong>\<^sub>Q c \<rbrakk
   by (simp add: qequiv_def)
 
 theorem qeq_iff_same_dim:
-  fixes x y :: "'a['u::dim_type]"
+  fixes x y :: "'a['d::dim_type]"
   shows "x \<cong>\<^sub>Q y \<longleftrightarrow> x = y"
   by (transfer, simp)
 
 (* the following series of equivalent statements ... *)
 
 lemma coerceQuant_eq_iff:
-  fixes x :: "'a['u\<^sub>1::dim_type]"
-  assumes "QD('u\<^sub>1) = QD('u\<^sub>2::dim_type)"
-  shows "(coerceQuantT TYPE('u\<^sub>2) x) \<cong>\<^sub>Q x"
+  fixes x :: "'a['d\<^sub>1::dim_type]"
+  assumes "QD('d\<^sub>1) = QD('d\<^sub>2::dim_type)"
+  shows "(coerceQuantT TYPE('d\<^sub>2) x) \<cong>\<^sub>Q x"
   by (metis qequiv.rep_eq assms coerceQuantT_def toQ_cases toQ_inverse)
 
 (* or equivalently *)
 
 lemma coerceQuant_eq_iff2:
-  fixes x :: "'a['u\<^sub>1::dim_type]"
-  assumes "QD('u\<^sub>1) = QD('u\<^sub>2::dim_type)" and "y = (coerceQuantT TYPE('u\<^sub>2) x)"
+  fixes x :: "'a['d\<^sub>1::dim_type]"
+  assumes "QD('d\<^sub>1) = QD('d\<^sub>2::dim_type)" and "y = (coerceQuantT TYPE('d\<^sub>2) x)"
   shows "x \<cong>\<^sub>Q y"
   using qequiv_sym assms(1) assms(2) coerceQuant_eq_iff by blast
  
 lemma updown_eq_iff:
-  fixes x :: "'a['u\<^sub>1::dim_type]" fixes y :: "'a['u\<^sub>2::dim_type]"
-  assumes "QD('u\<^sub>1) = QD('u\<^sub>2::dim_type)" and "y = (toQ (fromQ x))"
+  fixes x :: "'a['d\<^sub>1::dim_type]" fixes y :: "'a['d\<^sub>2::dim_type]"
+  assumes "QD('d\<^sub>1) = QD('d\<^sub>2::dim_type)" and "y = (toQ (fromQ x))"
   shows "x \<cong>\<^sub>Q y"
   by (simp add: assms(1) assms(2) coerceQuant_eq_iff2 coerceQuantT_def)
 
 text\<open>This is more general that \<open>y = x \<Longrightarrow> x \<cong>\<^sub>Q y\<close>, since x and y may have different type.\<close>
 
 lemma qeq: 
-  fixes x :: "'a['u\<^sub>1::dim_type]" fixes y :: "'a['u\<^sub>2::dim_type]"
+  fixes x :: "'a['d\<^sub>1::dim_type]" fixes y :: "'a['d\<^sub>2::dim_type]"
   assumes  "x \<cong>\<^sub>Q y"
-  shows "QD('u\<^sub>1) = QD('u\<^sub>2::dim_type)"
+  shows "QD('d\<^sub>1) = QD('d\<^sub>2::dim_type)"
   by (metis (full_types) qequiv.rep_eq assms fromQ mem_Collect_eq)
 
 subsection\<open>Operations on Abstract SI-Unit-Types\<close>
 
 lift_definition 
-  qtimes :: "('n::comm_ring_1)['a::dim_type] \<Rightarrow> 'n['b::dim_type] \<Rightarrow> 'n['a \<cdot>'b]" (infixl "\<^bold>\<cdot>" 69) is "(*)"
-  by (simp add: dim_ty_sem_DimTimes_def times_Quantity_ext_def)
+  qtimes :: "('n::comm_ring_1)['a::dim_type] \<Rightarrow> 'n['b::dim_type] \<Rightarrow> 'n['a \<cdot>'b]" (infixl "\<^bold>\<cdot>" 69) 
+  is "(*)" by (simp add: dim_ty_sem_DimTimes_def times_Quantity_ext_def)
   
 lift_definition 
-  qinverse :: "('n::field)['a::dim_type] \<Rightarrow> 'n['a\<^sup>-\<^sup>1]" ("(_\<^sup>-\<^sup>\<one>)" [999] 999) is "inverse"
-  by (simp add: inverse_Quantity_ext_def dim_ty_sem_DimInv_def)
+  qinverse :: "('n::field)['a::dim_type] \<Rightarrow> 'n['a\<^sup>-\<^sup>1]" ("(_\<^sup>-\<^sup>\<one>)" [999] 999) 
+  is "inverse" by (simp add: inverse_Quantity_ext_def dim_ty_sem_DimInv_def)
 
 abbreviation 
   qdivide :: "('n::field)['a::dim_type] \<Rightarrow> 'n['b::dim_type] \<Rightarrow> 'n['a/'b]" (infixl "\<^bold>'/" 70) where
@@ -257,8 +307,8 @@ end
 
 text\<open>The scaling operator permits to multiply the magnitude of a unit; this scalar product 
 produces what is called "prefixes" in the terminology of the SI system.\<close>
-lift_definition scaleQ :: "'a \<Rightarrow> 'a::comm_ring_1['u::dim_type] \<Rightarrow> 'a['u]" (infixr "*\<^sub>Q" 63)
-  is "\<lambda> r x. \<lparr> mag = r * mag x, dim = QD('u) \<rparr>" by simp
+lift_definition scaleQ :: "'a \<Rightarrow> 'a::comm_ring_1['d::dim_type] \<Rightarrow> 'a['d]" (infixr "*\<^sub>Q" 63)
+  is "\<lambda> r x. \<lparr> mag = r * mag x, dim = QD('d) \<rparr>" by simp
 
 notation scaleQ (infixr "\<odot>" 63)
 
